Restructure reachablility hints.
This specifies what types of hints the user would have to actually give.
We narrow up the hints to just have the user give jump address locations
for each possible expressions (or a "symbolic" location if the user is
sure that the code jumps to a non-program area). This also puts less
burden on the user to prove their hints' correctness.

We also merge the reachability and tracing computation into one single
function (since we now have a binary tree data structure to query known
reachable addresses) to simplify some of the code. By doing this, the
user also has the ability to query the store deltas of an address to
query the known current CPU state at that expression/instruction/address.

Finally, we added more modular arithmetic proofs and to help us prove
memory preservation. This creates a new type of memory-frame
preservation with the goal proving the minimum absolute distance away
from some target address. Doing so allows us to not have to destruct on
whether an address access overflows the address space (allowing us to
reduce the number of preconditions).

Picinae_calling.v
@@ -81,8 +81,8 @@ Next Obligation. Proof. decide equality. apply iseq. Defined.
 Definition store_delta := list (var * option exp).
 
 (* Convert a list of variables and their values to a store function. *)
-Fixpoint updlst s (l: store_delta) : var ⇀ exp :=
-  match l with nil => s | (v,u)::t => update (updlst s t) v u end.
+Fixpoint delta_updlst s (l: store_delta) : var ⇀ exp :=
+  match l with nil => s | (v,e)::t => update (delta_updlst s t) v e end.
 
 (* Remove a variable from a list of variables and their values. *)
 Fixpoint remlst v (l: store_delta) : store_delta :=
@@ -97,34 +97,37 @@ Notation "f [[ x := y ]]" := (setlst f x y) (at level 50, left associativity).
 Definition vdomain := var -> bool.
 Definition init_delta (domain: vdomain): var ⇀ exp := fun v =>
   if domain v then Some (Var v) else None.
-Notation "f << domain >> [[ x ]]" :=
-  (updlst (init_delta domain) f x)
+Notation "f <{ domain }> [[ x ]]" :=
+  (delta_updlst (init_delta domain) f x)
   (at level 50, left associativity).
 
+Definition trim_delta_state (vd: vdomain) (δ: store_delta) :=
+  flat_map (fun '(v, e) => if vd v then (v, e) :: nil else nil) δ.
+
 Definition has_delta (vd: vdomain) (h: hdomain) (s0 s: store) (δ: store_delta) :=
-  forall v e val (LUv: δ<<vd>>[[v]] = Some e) (EE: eval_exp h s0 e val), s v = val.
+  forall v e val (LUv: δ<{vd}>[[v]] = Some e) (EE: eval_exp h s0 e val), s v = val.
 
 Definition delta_nounk (vd: vdomain) (δ: store_delta) :=
-  forall v e (LUv: δ<<vd>>[[v]] = Some e), forall_exps_in_exp not_unknown e.
+  forall v e (LUv: δ<{vd}>[[v]] = Some e), forall_exps_in_exp not_unknown e.
 
 Definition delta_defined (δ: store_delta) :=
   map fst δ.
 
 Definition delta_equivb (vd: vdomain) (δ1 δ2: store_delta) :=
-  forallb (fun '(v, _) => iseqb (δ1<<vd>>[[v]]) (δ2<<vd>>[[v]])) (δ1 ++ δ2).
+  forallb (fun '(v, _) => iseqb (δ1<{vd}>[[v]]) (δ2<{vd}>[[v]])) (δ1 ++ δ2).
 
 Definition delta_equiv (vd: vdomain) (δ1 δ2: store_delta) :=
-  forall v, δ1<<vd>>[[v]] = δ2<<vd>>[[v]].
+  forall v, δ1<{vd}>[[v]] = δ2<{vd}>[[v]].
 
 Definition delta_same_domain (vd: vdomain) (δ1 δ2: store_delta) :=
-  forall v, match (δ1<<vd>>[[v]]), (δ2<<vd>>[[v]]) with
+  forall v, match (δ1<{vd}>[[v]]), (δ2<{vd}>[[v]]) with
             | Some _, Some _ => True
             | None, None => True
             | _, _ => False
             end.
 
-Theorem updlst_def: forall f δ v (ND: ~(In v (delta_defined δ))),
-  updlst f δ v = f v.
+Theorem delta_updlst_def: forall f δ v (ND: ~(In v (delta_defined δ))),
+  delta_updlst f δ v = f v.
 Proof.
   induction δ; intros.
   - reflexivity.
@@ -139,16 +142,16 @@ Proof.
 Qed.
 
 Theorem delta_remlst_removed: forall δ fn v,
-  updlst fn (remlst v δ) v = fn v.
+  delta_updlst fn (remlst v δ) v = fn v.
 Proof.
-  intros. apply updlst_def. intros Contra. revert v Contra. induction δ; intros. 
+  intros. apply delta_updlst_def. intros Contra. revert v Contra. induction δ; intros. 
   - inversion Contra.
   - simpl in Contra. destruct a as [v' u']. eapply IHδ. destruct (v == v').
     eassumption. apply neq_sym in n. destruct Contra; [contradiction n|assumption].
 Qed.
 
 Theorem delta_remlst_frame: forall δ fn x z (NEQ: z ≠ x),
-  updlst fn (remlst x δ) z = updlst fn δ z.
+  delta_updlst fn (remlst x δ) z = delta_updlst fn δ z.
 Proof.
   induction δ; intros.
   - reflexivity.
@@ -160,18 +163,18 @@ Proof.
       apply IHδ. assumption.
 Qed.
 
-Theorem delta_update_updated: forall fn δ x y, updlst fn (δ [[x := y]]) x = y.
+Theorem delta_update_updated: forall fn δ x y, delta_updlst fn (δ [[x := y]]) x = y.
 Proof. intros. unfold setlst. simpl. apply update_updated. Qed.
 
 Theorem delta_update_frame: forall δ fn x y z (NEQ: z ≠ x),
-  updlst fn (δ [[x := y]]) z = updlst fn δ z.
+  delta_updlst fn (δ [[x := y]]) z = delta_updlst fn δ z.
 Proof.
   intros. unfold setlst. simpl. rewrite update_frame by assumption.
   apply delta_remlst_frame. assumption.
 Qed.
 
-Theorem delta_updlst_iff_defined: forall f δ v,
-  In v (delta_defined δ) <-> In (v, updlst f δ v) δ.
+Theorem delta_delta_updlst_iff_defined: forall f δ v,
+  In v (delta_defined δ) <-> In (v, delta_updlst f δ v) δ.
 Proof.
   split.
   - intro InDef. revert_all. induction δ; intros.
@@ -188,25 +191,25 @@ Proof.
         right. apply IHδ. rewrite update_frame in H; assumption.
 Qed.
 
-Corollary delta_updlst_iff_defined_contra: forall f δ v,
-  ~ In v (delta_defined δ) <-> ~ In (v, updlst f δ v) δ.
-Proof. intros. contrapositive delta_updlst_iff_defined. Qed.
+Corollary delta_delta_updlst_iff_defined_contra: forall f δ v,
+  ~ In v (delta_defined δ) <-> ~ In (v, delta_updlst f δ v) δ.
+Proof. intros. contrapositive delta_delta_updlst_iff_defined. Qed.
 
 Theorem delta_equivb_iff_delta_equiv: forall vd δ1 δ2,
   delta_equivb vd δ1 δ2 = true <-> delta_equiv vd δ1 δ2.
 Proof.
   unfold delta_equiv, delta_equivb. split; intro EQV.
   - (* -> *) intro. rewrite forallb_app, andb_true_iff in EQV.
-    destruct EQV as [EQV1 EQV2]. edestruct (in_dec iseq (v, δ1<<vd>>[[v]])).
+    destruct EQV as [EQV1 EQV2]. edestruct (in_dec iseq (v, δ1<{vd}>[[v]])).
     + eapply forallb_forall in EQV1; [|eassumption]. simpl in EQV1.
       unfold iseqb in EQV1. destruct (_ == _); try discriminate. assumption.
-    + edestruct (in_dec iseq (v, δ2<<vd>>[[v]])).
+    + edestruct (in_dec iseq (v, δ2<{vd}>[[v]])).
       * eapply forallb_forall in EQV2; [|eassumption]. simpl in EQV2.
         unfold iseqb in EQV2. destruct (_ == _); try discriminate. assumption.
-      * repeat rewrite updlst_def; try rewrite delta_updlst_iff_defined_contra;
+      * repeat rewrite delta_updlst_def; try rewrite delta_delta_updlst_iff_defined_contra;
         trivial2.
   - (* <- *) rewrite forallb_forall. intros. destruct x as [v e]. rewrite EQV.
-    unfold iseqb. vreflexivity (δ2<<vd>>[[v]]). reflexivity.
+    unfold iseqb. vreflexivity (δ2<{vd}>[[v]]). reflexivity.
 Qed.
 
 Corollary delta_equivb_iff_delta_equiv_contra: forall vd δ1 δ2,
@@ -214,6 +217,33 @@ Corollary delta_equivb_iff_delta_equiv_contra: forall vd δ1 δ2,
 Proof.
   intros. rewrite <- not_true_iff_false.
   contrapositive delta_equivb_iff_delta_equiv.
+Qed.
+
+Lemma trim_delta_state_preserve: forall vd δ v
+  (VD: vd v = true), trim_delta_state vd δ <{vd}>[[v]] = δ<{vd}>[[v]].
+Proof.
+  induction δ; intros.
+  - reflexivity.
+  - destruct a as [v' e']. simpl. destruct (v == v').
+    + subst. rewrite VD. simpl. repeat rewrite update_updated.
+      reflexivity.
+    + einstantiate trivial IHδ. destruct (vd v'); simpl;
+      repeat rewrite update_frame; assumption.
+Qed.
+
+Theorem trim_delta_state_correct: forall vd δ h s0 s
+  (HD: has_delta vd h s0 s δ), has_delta vd h s0 s (trim_delta_state vd δ).
+Proof.
+  unfold has_delta. intros. destruct (vd v) eqn: VD.
+  - rewrite trim_delta_state_preserve in LUv by assumption.
+    eapply HD; eassumption.
+  - unfold trim_delta_state, init_delta in LUv. rewrite delta_updlst_def, VD in LUv.
+    discriminate. intro InMap. unfold delta_defined in InMap.
+    rewrite flat_map_concat_map, concat_map, map_map,
+      <- flat_map_concat_map, in_flat_map in InMap.
+    destruct InMap as [ [v' e'] [InDelta InVD] ].
+    destruct (vd v') eqn: VD'; inversion InVD; subst; try inversion H.
+    simpl in *. rewrite VD in VD'. discriminate.
 Qed.
 
 Lemma models_assign: forall c h s v e u t (MDL: models c s)
@@ -269,7 +299,7 @@ Qed.
 Theorem delta_same_domain_refl: forall vd δ, delta_same_domain vd δ δ.
 Proof.
   unfold delta_same_domain. intros.
-  destruct (δ<<vd>>[[v]]); reflexivity.
+  destruct (δ<{vd}>[[v]]); reflexivity.
 Qed.
 
 Theorem delta_same_domain_assign: forall vd v δ1 δ2 o1 o2
@@ -290,7 +320,7 @@ Qed.
 Fixpoint subst_valid (vd: vdomain) (δ: store_delta) e: bool :=
   match e with
   | Var v =>
-      match δ<<vd>>[[v]] with
+      match δ<{vd}>[[v]] with
       | Some e => true
       | None => false
       end
@@ -313,7 +343,7 @@ Fixpoint subst_valid (vd: vdomain) (δ: store_delta) e: bool :=
 Fixpoint subst_exp0 (vd: vdomain) (δ: store_delta) e: exp :=
   match e with
   | Var v =>
-      match δ<<vd>>[[v]] with
+      match δ<{vd}>[[v]] with
       | Some e => e
       | None => Unknown 0 (* Note we should return error in subst_err here *)
       end
@@ -345,7 +375,7 @@ Proof.
   try erewrite IHe2 by eassumption; try erewrite IHe3 by eassumption;
   try erewrite IHe by eassumption; try reflexivity.
 
-  (* Var *) specialize (DSD v). destruct (δ1<<vd>>[[v]]), (δ2<<vd>>[[v]]);
+  (* Var *) specialize (DSD v). destruct (δ1<{vd}>[[v]]), (δ2<{vd}>[[v]]);
   try solve [contradiction DSD|reflexivity].
 
   (* Let *) destruct subst_valid eqn: SV1; erewrite IHe2; try reflexivity;
@@ -377,7 +407,7 @@ Theorem subst_exp0_nounk: forall vd e δ (DNU: delta_nounk vd δ)
 Proof.
   unfold subst_exp; induction e; intros; simpl in SE;
   try solve [exp_destruction_nounk; repeat split; assumption + reflexivity].
-  - (* Var *) destruct (δ<<vd>>[[v]]) eqn: LUv; inversion SE. subst. eapply DNU.
+  - (* Var *) destruct (δ<{vd}>[[v]]) eqn: LUv; inversion SE. subst. eapply DNU.
     simpl. rewrite LUv. reflexivity.
   - (* Let *) simpl. destruct subst_valid eqn: SV1.
     + (* e1 is valid *) apply IHe2. apply delta_nounk_assign_Some. assumption.
@@ -427,7 +457,7 @@ Proof.
 
   unfold subst_exp; induction e; intros; inversion EE; subst;
   simpl in SE; clear EE; try solve [exp_destruction_correct; reflexivity].
-  - (* Var *) destruct (δ<<vd>>[[v]]) eqn: LUv; inversion SE. subst. erewrite HD;
+  - (* Var *) destruct (δ<{vd}>[[v]]) eqn: LUv; inversion SE. subst. erewrite HD;
     solve [reflexivity|eassumption].
   - (* Let *) destruct subst_valid eqn: SV1.
     + (* e1 is valid *) erewrite subst_valid_any_Some in SE. eapply IHe2;
@@ -444,13 +474,44 @@ Qed.
 
 Definition trace_states := treeN store_delta.
 
-  (*
- * list addr)%type.
-Definition trace_states_prop := (trace_states * (var -> option Prop))%type.
-   *)
-Definition trace_state_res := option (list (store_delta * option exit)).
-Definition trace_state_res_with_prop :=
-  option (list (store_delta * option exit) * (var -> option Prop)).
+Inductive jump_target: Set :=
+  | jump_addr (a: addr)
+  | jump_symbolic. (* a call or return *)
+
+
+Inductive eval_jump (p: program) (s: store):
+  addr -> jump_target -> Prop :=
+  | EJ_jump_addr (a: addr): eval_jump p s a (jump_addr a)
+  | EJ_jump_symbolic (a: addr) (LU: p s a = None):
+      eval_jump p s a jump_symbolic.
+
+Definition eval_jump_targets p s a (jmps: list jump_target): Prop :=
+  Exists (eval_jump p s a) jmps.
+
+Inductive ts_evidence :=
+  | has_jump_targets (a1: addr) (q0: stmt) (δ: store_delta) (vd: vdomain)
+      (e: exp) (jmps: list jump_target).
+
+Inductive ts_evidence_proved (p: program) (h: hdomain)
+  (a0: addr) (s0: store): ts_evidence -> Prop :=
+  | EV_has_jump_targets (a1: addr) (q0: stmt) (δ: store_delta)
+      (vd: vdomain) (e: exp) (jmps: list jump_target) (EJT: forall n a' s0' s1
+        (XP: exec_prog h p a0 s0 n s0' (Exit a1))
+        (XS0: exec_stmt h s0' q0 s1 None)
+        (XS: exec_stmt h s1 (Jmp e) s1 (Some (Exit a')))
+        (HD: has_delta vd h s0 s1 δ),
+        eval_jump_targets p s1 a' jmps):
+        ts_evidence_proved p h a0 s0 (has_jump_targets a1 q0 δ vd e jmps).
+
+Definition trace_state_res :=
+  option (list (store_delta * option exit) * list ts_evidence).
+
+Definition sat_evidences (evs: list ts_evidence) p h a0 s0 :=
+  Forall (ts_evidence_proved p h a0 s0) evs.
+
+(* TODO: remove redundant ts_evidences *)
+Definition app_evidences (ev1 ev2: list ts_evidence) := ev1 ++ ev2.
+Notation "ev1 !++ ev2" := (app_evidences ev1 ev2) (at level 60, right associativity).
 
 Fixpoint map_option {A B} (f: A -> option B) (l: list A): option (list B) :=
   match l with
@@ -519,94 +580,155 @@ Proof.
     + simpl. erewrite IHl; try eassumption. destruct (f a); reflexivity.
 Qed.
 
-Fixpoint simple_trace_stmt (vd: vdomain) (δ: store_delta) (q: stmt):
-  trace_state_res :=
+Definition jump_hint := addr -> store_delta -> exp -> option (list jump_target).
+
+Fixpoint simple_trace_stmt0 (hint: jump_hint) (vd: vdomain) (δ: store_delta)
+  (a: addr) (q0: stmt) (q: stmt): trace_state_res :=
   match q with
-  | Nop => Some ((δ, None) :: nil)
-  | Move v e => Some
-      ((if vd v then δ[[v := subst_exp vd δ e]] else remlst v δ, None) :: nil)
+  | Nop => Some ((δ, None) :: nil, nil)
+  | Move v e => Some ((δ[[v := subst_exp vd δ e]], None) :: nil, nil)
   | Jmp e =>
-      match subst_exp vd δ e with
-      | Some (Word n _) => Some ((δ, Some (Exit n)) :: nil)
-      | _ => None
+      match hint a δ e with
+      | Some jmps =>
+          Some (flat_map (fun j =>
+            match j with
+            | jump_addr a => ((δ, Some (Exit a)) :: nil)
+            | jump_symbolic => nil
+            end) jmps, has_jump_targets a q0 δ vd e jmps :: nil)
+      | None =>
+          match subst_exp vd δ e with
+          | Some (Word n _) => Some ((δ, Some (Exit n)) :: nil, nil)
+          | _ => None
+          end
       end
-  | Exn n => Some ((δ, Some (Raise n)) :: nil)
+  | Exn n => Some ((δ, Some (Raise n)) :: nil, nil)
   | Seq q1 q2 =>
-      match simple_trace_stmt vd δ q1 with
+      match simple_trace_stmt0 hint vd δ a q0 q1 with
       | None => None
-      | Some paths1 =>
+      | Some (paths1, ev1) =>
           let res := map_option (fun '(δ', x) =>
             match x with
             | None =>
-                match simple_trace_stmt vd δ' q2 with
+                match simple_trace_stmt0 hint vd δ' a (Seq q0 q1) q2 with
                 | None => None
-                | Some paths2 => Some paths2
+                | Some (paths2, _) => Some paths2
                 end
             | Some _ => Some ((δ', x) :: nil)
             end) paths1 in
+          let ev' := flat_map (fun '(δ', x) =>
+            match x with
+            | None =>
+                match simple_trace_stmt0 hint vd δ' a (Seq q0 q1) q2 with
+                | None => nil
+                | Some (_, ev2) => ev2
+                end
+            | Some _ => nil
+            end) paths1 !++ ev1 in
           match res with
           | None => None
-          | Some ll => Some (concat ll)
+          | Some ll => Some (concat ll, ev')
           end
       end
   | If _ q1 q2 =>
-      match simple_trace_stmt vd δ q1, simple_trace_stmt vd δ q2 with
+      match simple_trace_stmt0 hint vd δ a q0 q1, simple_trace_stmt0 hint vd δ a q0 q2 with
       | None, _ | _, None => None
-      | Some paths1, Some paths2 =>
-          Some (paths1 ++ paths2)
+      | Some (paths1, ev1), Some (paths2, ev2) =>
+          Some (paths1 ++ paths2, ev1 !++ ev2)
       end
   | Rep _ s => None
   end.
 
-Theorem simple_trace_stmt_correct: forall vd s0 q paths h s s' x δ
-  (HD: has_delta vd h s0 s δ) (XS: exec_stmt h s q s' x)
-  (STS: simple_trace_stmt vd δ q = Some paths),
-  Exists (fun '(δ', x') => x' = x /\ has_delta vd h s0 s' δ') paths.
+Theorem simple_trace_stmt0_correct: forall hints vd q q0 paths h p n
+  a0 s0 s0' a1 s1 x2 s2 δ evs
+  (HD: has_delta vd h s0 s1 δ) (XS: exec_stmt h s1 q s2 x2)
+  (LU2: forall a2, x2 = Some (Exit a2) -> exists insn, p s2 a2 = Some insn)
+  (STS: simple_trace_stmt0 hints vd δ a1 q0 q = Some (paths, evs))
+  (XP: exec_prog h p a0 s0 n s0' (Exit a1)) (XS0: exec_stmt h s0' q0 s1 None)
+  (EV: sat_evidences evs p h a0 s0),
+  Exists (fun '(δ', x') => x' = x2 /\ has_delta vd h s0 s2 δ') paths.
 Proof.
-  induction q; intros; inversion XS; inversion STS; subst; clear XS STS.
-  - (* Nop *) constructor. split. reflexivity. assumption.
-  - (* Move *) constructor. split. reflexivity. destruct vd eqn: VD.
-    + destruct subst_exp eqn: SE1; [|apply has_delta_assign_None; assumption]. 
-      apply has_delta_assign_Some. assumption. intros.
-      eapply subst_exp_correct; eassumption.
-    + unfold has_delta. intros. destruct (v0 == v).
-      * subst. unfold init_delta in LUv. rewrite delta_remlst_removed, VD in LUv.
-        discriminate.
-      * rewrite update_frame by assumption. rewrite delta_remlst_frame in LUv by assumption.
-        eapply HD; eassumption.
-  - (* Jmp *) destruct (subst_exp _ _ _) eqn: SE; try destruct e0; inversion H3.
-    subst. constructor. split; try assumption.
-    einstantiate trivial subst_exp_correct as Res. constructor. inversion Res.
-    reflexivity.
-  - (* Exn *) constructor. split. reflexivity. assumption.
-  - (* Seq, exit 1 *) destruct simple_trace_stmt as [paths1|] eqn: SQ1; try discriminate.
-    einstantiate trivial (IHq1). destruct map_option eqn: Map; inversion H4.
-    subst. clear H4. rename l into paths_res. apply Exists_exists in H.
+  induction q; intros; inversion XS; inversion STS; subst; clear STS.
+  - (* Nop *) constructor. split; trivial2.
+  - (* Move *) constructor. split. reflexivity. destruct subst_exp eqn: SE1;
+    [|apply has_delta_assign_None; assumption]. apply has_delta_assign_Some.
+    assumption. intros. eapply subst_exp_correct; eassumption.
+  - (* Jmp *) destruct hints as [jmps|].
+    + (* Use hint *) inversion H3. subst. clear H3. inversion EV. inversion H1.
+      subst. einstantiate trivial EJT as EJT. apply Exists_exists in EJT.
+      apply Exists_exists. einversion trivial LU2 as [insn LU'].
+      destruct EJT as [j [InJmps EJ] ]. inversion EJ;
+      [|rewrite LU in LU'; discriminate]. subst. clear EJ.
+      eexists. split. apply in_flat_map. eexists. split; [eassumption|].
+      simpl. left. reflexivity. simpl. split; trivial2.
+    + (* No hint *) destruct (subst_exp _ _ _) eqn: SE; try destruct e0; inversion H3.
+      subst. constructor. split; [|assumption].
+      einstantiate trivial subst_exp_correct as Res. constructor. inversion Res.
+      subst. reflexivity.
+  - (* Exn *) constructor. split; trivial2.
+  - (* Seq, exit 1 *) destruct simple_trace_stmt0 as [res1|] eqn: SQ1; try discriminate.
+    destruct res1 as [paths1 ev1]. destruct map_option as [path_res|] eqn: Map;
+    inversion H4. subst. clear XS H4. apply Forall_app in EV.
+    destruct EV as [EV EV1]. einstantiate trivial IHq1. apply Exists_exists in H.
     destruct H as [ [δ1 x1] [InP1 [X HD1] ] ]; subst. apply Exists_exists.
-    exists (δ1, Some x0). repeat split; [|assumption]. apply in_concat. eexists.
-    split; [|apply in_eq]. eapply map_option_includes; try eassumption.
-    reflexivity.
-  - (* Seq, exit 2 *) destruct (simple_trace_stmt) eqn:SQ1; [|discriminate].
-    destruct map_option eqn:MO; inversion H4. subst. clear H4. einstantiate
-    trivial IHq1. apply Exists_exists in H. apply Exists_exists.
-    destruct H as [ [δ1 x1] [InP1 [X HD1] ] ]. subst.
-    destruct (simple_trace_stmt vd δ1 q2) eqn:SQ2.
-    + einstantiate IHq2 as IHq2; try assumption; try apply SQ2; try apply TS2;
-      try apply XS0; try eassumption. apply Exists_exists in IHq2.
-      destruct IHq2 as [ [δ' x'] [Inl1 HD'] ]. eexists. split.
+    exists (δ1, Some x). repeat split; try assumption. apply in_concat. eexists.
+    split; [|apply in_eq].  eapply map_option_includes; try eassumption. reflexivity.
+  - (* Seq, exit 2 *) destruct simple_trace_stmt0 as [res1|] eqn:SQ1; [|discriminate].
+    destruct res1 as [paths1 ev1]. destruct map_option as [path_res|] eqn: Map;
+    inversion H4. subst. clear XS H4. apply Forall_app in EV. destruct EV as [EV EV1].
+    einstantiate trivial IHq1. apply Exists_exists in H.
+    destruct H as [ [δ1 x1] [InP1 [X HD1] ] ]; subst. apply Exists_exists.
+    destruct (simple_trace_stmt0 hints vd δ1 a1 (q0 $; q1) q2) as [ [paths2 ev2]|] eqn:SQ2.
+    + (* Expand out IHq2. We have to show that ev2 is part of ev' *)
+      einstantiate trivial IHq2 as IHq2. econstructor; eassumption.
+      unfold sat_evidences. rewrite Forall_forall in *. intros ev' InEV2.
+      einstantiate trivial EV. apply in_flat_map. eexists. split. eassumption.
+      simpl. rewrite SQ2. eassumption. rewrite Exists_exists in IHq2.
+      destruct IHq2 as [ [δ' x'] [InP2 [EQ HD'] ] ]. subst.
 
-      (* Prove that state is in concat l0 *) apply in_concat. eexists.
-      split; try eassumption. eapply map_option_includes; try eassumption.
-      simpl. rewrite SQ2. reflexivity. simpl. assumption.
-    + erewrite map_option_fails in MO; try solve [discriminate|eassumption].
+      (* From IHq2, show that delta holds since the state is in (concat path_res) *)
+      eexists. split. apply in_concat. eexists. split; [|eassumption].
+      eapply map_option_includes; try eassumption. simpl. rewrite SQ2.
+      reflexivity. simpl. split; trivial2.
+    + erewrite map_option_fails in Map; try solve [discriminate|eassumption].
       simpl. rewrite SQ2. reflexivity.
   - (* If/else *) destruct c;
-    (destruct (simple_trace_stmt) eqn: ST1; [|discriminate]);
-    (destruct (simple_trace_stmt vd δ q2) eqn: ST2; [|discriminate]).
+    (destruct (simple_trace_stmt0) as [ [paths1 ev1]|] eqn: ST1; [|discriminate]);
+    (destruct (simple_trace_stmt0 _ _ _ _ _ q2) as [ [paths2 ev2]|] eqn: ST2;
+        [|discriminate]); inversion H5; subst; apply Forall_app in EV;
+    destruct EV.
     + (* q2 *) einstantiate trivial IHq2. eapply incl_Exists.
-      inversion H5. apply incl_appr. apply incl_refl. assumption.
+      apply incl_appr. apply incl_refl. assumption.
     + (* q1 *) einstantiate trivial IHq1. eapply incl_Exists.
-      inversion H5. apply incl_appl. apply incl_refl. assumption.
+      apply incl_appl. apply incl_refl. assumption.
+Qed.
+
+Definition simple_trace_stmt (hint: jump_hint) (vd: vdomain) (δ: store_delta)
+  (a: addr) (q: stmt): trace_state_res :=
+  match simple_trace_stmt0 hint vd δ a Nop q with
+  | Some (next_states, evs) =>
+      Some (map (fun '(δ, x) => (trim_delta_state vd δ, x)) next_states, evs)
+  | None => None
+  end.
+
+Theorem simple_trace_stmt_correct: forall hints vd q paths h p n
+  a0 s0 a1 s1 x2 s2 δ evs (XP: exec_prog h p a0 s0 n s1 (Exit a1))
+  (HD: has_delta vd h s0 s1 δ) (XS: exec_stmt h s1 q s2 x2)
+  (LU2: match x2 with
+        | Some (Exit a2) => exists insn, p s2 a2 = Some insn
+        | _ => True
+        end)
+  (STS: simple_trace_stmt hints vd δ a1 q = Some (paths, evs))
+  (EV: sat_evidences evs p h a0 s0),
+  Exists (fun '(δ', x') => x' = x2 /\ has_delta vd h s0 s2 δ') paths.
+Proof.
+  intros. unfold simple_trace_stmt in STS.
+  destruct simple_trace_stmt0 as [ [next_states evs']|] eqn: STS0; try discriminate.
+  inversion STS. subst. clear STS. einstantiate trivial simple_trace_stmt0_correct.
+  intros. subst. assumption. constructor. rewrite Exists_exists in *.
+  destruct H as [ [δ' x'] [InX [EQ HD0] ] ]. subst.
+  eexists (_, x2). repeat split. eassert (X: (_, x2) = _ _);
+    [|rewrite X; apply in_map; eassumption]. reflexivity.
+  apply trim_delta_state_correct. assumption.
 Qed.
 
 Definition join_states_if_changed (vd: vdomain) (δ1: option store_delta)
@@ -616,28 +738,16 @@ Definition join_states_if_changed (vd: vdomain) (δ1: option store_delta)
       if delta_equivb vd δ1 δ2
       then None
       else let δ_merge := (fold_right (fun v δ' =>
-        δ'[[v := if δ1<<vd>>[[v]] == δ2<<vd>>[[v]] then δ2<<vd>>[[v]] else None]])
+        δ'[[v := if δ1<{vd}>[[v]] == δ2<{vd}>[[v]] then δ2<{vd}>[[v]] else None]])
         nil (delta_defined (δ1 ++ δ2))) in
         if delta_equivb vd δ1 δ_merge then
             None
         else
-            Some δ_merge 
+            Some δ_merge
   | None => Some δ2
   end.
 
 Definition null_state: store := fun _ => VaN 0 0.
-
-Definition h_conj h1 h2 := fun (v: var) =>
-  match h1 v, h2 v with
-  | None, p | p, None => p
-  | Some p1, Some p2 => Some (p1 /\ p2)
-  end.
-
-Definition true_hyp {V} hyps (v:V) :=
-  match hyps v with
-  | Some hyp => hyp
-  | None => True
-  end.
 
 Definition process_state (vd: vdomain) (exitof: option exit -> exit)
   (st: store_delta * option exit) (accum: trace_states * bool) :=
@@ -668,62 +778,53 @@ Definition correctness_sub_prog vd p domain ts h a0 s0 :=
     (TS2: tget_n ts a1 = Some δ), has_delta vd h s0 s1 δ).
 
 Definition trace_program_step_at (vd: vdomain) (p: program)
-  (hints: program -> addr -> trace_states -> option (trace_states * bool))
-  addr (accum: option (trace_states * bool)) :=
+  (hints: jump_hint) addr (accum: option (trace_states * bool * list ts_evidence)) :=
   match accum with
   | None => None
-  | Some (ts, changed) =>
-      (* Use hints if we have information *)
-      match hints p addr ts with
-      | None =>
-          (* If this is a proper address in program, process that. *)
-          match p null_state addr with
-          (* TODO: some logic saying that for all possible executions that there
-           * exists some point later on in this execution such that it matches
-           * one of the store deltas that we recorded. *)
-          | None => None (*Some (ts, working, P)*)
-          | Some (sz, q) =>
-              (* Sanity check for if we have already visited this address *)
-              match tget_n ts addr with
-              | None => Some (ts, changed)
-              | Some δ_a =>
-                  match simple_trace_stmt vd δ_a q with
-                  | None => None
-                  | Some next_states =>
-                      let res := fold_right (process_state vd
-                        (exitof (addr + sz))) (ts, changed) next_states in
-                      Some res
-                  end
+  | Some (ts, changed, old_evs) =>
+      (* If this is a proper address in program, process that. Otherwise, this
+       * is an invalid execution, so wouldn't happen to begin with. *)
+      match p null_state addr with
+      | None => Some (ts, changed, old_evs)
+      | Some (sz, q) =>
+          (* We have to had visited this address to begin with; otherwise, we
+           * won't be able to push trace states for this address's successors. *)
+          match tget_n ts addr with
+          | None => Some (ts, changed, old_evs)
+          | Some δ_a =>
+              match simple_trace_stmt hints vd δ_a addr q with
+              | None => None
+              | Some (next_states, evs) =>
+                  let res := fold_right (process_state vd
+                    (exitof (addr + sz))) (ts, changed) next_states in
+                  Some (res, evs !++ old_evs)
               end
           end
-      | Some (ts', changed') => Some (ts', changed || changed')
       end
   end.
 
-Definition expand_trace_program (vd: vdomain) (p: program) 
-  (hints: program -> addr -> trace_states -> option (trace_states * bool))
-  (reachable: set) (init_ts: trace_states): option (trace_states * bool) :=
-  fold_right (trace_program_step_at vd p hints) (Some (init_ts, false))
-    (set_elems reachable).
+Definition expand_trace_program (vd: vdomain) (p: program)
+  (hints: jump_hint) (init_ts: trace_states):
+  option (trace_states * bool * list ts_evidence) :=
+  fold_right (trace_program_step_at vd p hints) (Some (init_ts, false, nil))
+    (tkeys_n init_ts).
 
 Definition iterM (n: N) {A} (f: A -> option A) (x: A) :=
   N.iter n (fun x => match x with Some x => f x | None => None end) (Some x).
 
 Definition expand_trace_program_n (n: N) (vd: vdomain)
-  (hints: program -> addr -> trace_states -> option (trace_states * bool))
-  (p: program) (reachable: set) (init_ts: trace_states):
-  option (trace_states * bool) :=
+  (hints: jump_hint) (p: program) (init_ts: trace_states):
+  option (trace_states * bool * list ts_evidence) :=
   N.iter n (fun x =>
     match x with
-    | Some (ts, true) => expand_trace_program vd p hints reachable ts
-    | Some (ts, false) => Some (ts, false)
+    | Some (ts, true, _) => expand_trace_program vd p hints ts
+    | Some (ts, false, ev) => Some (ts, false, ev)
     | None => None
-    end) (Some (init_ts, true)).
+    end) (Some (init_ts, true, nil)).
 
-Lemma fold_expand_trace_program: forall vd p hints reachable init_ts,
-  fold_right (trace_program_step_at vd p hints) (Some (init_ts, false))
-    (set_elems reachable) =
-  expand_trace_program vd p hints reachable init_ts.
+Lemma fold_expand_trace_program: forall vd p hints init_ts,
+  fold_right (trace_program_step_at vd p hints) (Some (init_ts, false, nil))
+    (tkeys_n init_ts) = expand_trace_program vd p hints init_ts.
 Proof. reflexivity. Qed.
 
 (*
@@ -1175,19 +1276,18 @@ Proof.
   Picinae_typecheck.
 Qed.
 
-Definition simp_prog_trace_hint (p: program) (a: addr) (ts: trace_states):
-  option (trace_states * bool) := None.
+Definition simp_prog_jump_hints: jump_hint := fun a δ e => None.
 
-Definition simp_prog_trace reachables := expand_trace_program_n 10 (fun _ => true)
-  simp_prog_trace_hint simp_prog reachables (tupdate_n treeN_nil 0 nil).
+Definition simp_prog_trace := expand_trace_program_n 10 (fun _ => true)
+  simp_prog_jump_hints simp_prog (tupdate_n treeN_nil 0 nil).
 
 Goal True.
 Proof.
 
-  pose (x := match simp_prog_trace {{0;1}} with
-             | Some (ts, b) =>
+  pose (x := match simp_prog_trace with
+             | Some (ts, b, ev) =>
                  match tget_n ts 1 with
-                 | Some δ => Some (ts, δ, b)
+                 | Some δ => Some (ts, δ, b, ev)
                  | None => None
                  end
              | None => None
@@ -1195,31 +1295,27 @@ Proof.
   compute in x.
 Abort.
 
-
-
+Require Import test.
 Theorem my_prog_welltyped: welltyped_prog x86typctx my_prog.
 Proof.
   Picinae_typecheck.
 Qed.
 
-Definition my_prog_reachables_hint (ret: addr) (a: addr): option set :=
+Definition my_prog_jump_hints: jump_hint := fun a δ e =>
   match a with
-  | 34 => Some {{ret}}
+  | 34 => Some (jump_symbolic :: nil)
   | _ => None
   end.
 
-Definition my_prog_reachables ret := expand_reachables_fast_n
-  (my_prog_reachables_hint ret) my_prog (0 :: nil, 0 :: nil) 100.
-
-Definition my_prog_trace_hint (p: program) (a: addr) (ts: trace_states):
-  option (trace_states * bool) :=
-  match a with
-  | 34 => Some (ts, false)
-  | _ => None
+Definition domain1 var :=
+  match var with
+  | V_TEMP _ => false
+  | R_AF | R_CF | R_DF | R_OF | R_PF | R_SF | R_ZF => false
+  | _ => true
   end.
 
-Definition my_prog_trace x reachables := expand_trace_program_n x (fun _ => true)
-  my_prog_trace_hint my_prog reachables (tupdate_n treeN_nil 0 nil).
+Definition my_prog_trace x := expand_trace_program_n x domain1
+  my_prog_jump_hints my_prog (tupdate_n treeN_nil 0 nil).
 
 Ltac unbox_res v :=
   match eval red in v with
@@ -1230,16 +1326,113 @@ Ltac unbox_Some v :=
   match eval red in v with
   | Some ?v' => clear v; pose (v := v')
   end.
-
-
-Goal True.
+Goal forall esp0 s0 (MDL0: models x86typctx s0)
+  (SV2: s0 R_ESP = Ⓓ esp0),
+  exists val,
+  eval_exp fh (s0 [ R_ESP := Ⓓ  42 ] [A_READ := Ⓜ (fun _ => 1)]
+    [A_WRITE := Ⓜ (fun _ => 1)])
+  (Load
+     (Store
+        (Store (Var V_MEM32) (BinOp OP_MINUS (Var R_ESP) (Word 4 32))
+           (Cast CAST_LOW 32 (Var R_EBP)) LittleE 4)
+        (BinOp OP_PLUS (BinOp OP_MINUS (Var R_ESP) (Word 4 32))
+           (Word 4294967292 32)) (Word 0 32) LittleE 4)
+     (BinOp OP_PLUS (BinOp OP_MINUS (Var R_ESP) (Word 4 32)) (Word 4 32))
+     LittleE 4) val.
 Proof.
+  intros.
+  assert (MDL': models x86typctx (s0 [ R_ESP := Ⓓ  42 ] [A_READ := Ⓜ (fun _ => 1)]
+    [A_WRITE := Ⓜ (fun _ => 1)])).
+    intros v t eq. destruct v; psimpl;
+    try solve [ eapply MDL0; eassumption
+              | einversion eq; constructor; try intro; reflexivity].
 
-  pose (reachables := my_prog_reachables 0).
-  compute in reachables. unbox_res reachables.
-  pose (x := my_prog_trace 100 (list_to_set reachables)). compute in x.
+  match goal with |- exists u, eval_exp ?h ?s ?e u =>
+      mk_eval_exp h s e EE
+  end.
 
-Abort.
+  repeat split; try reflexivity; unfold mem_readable, mem_writable; psimpl;
+  eexists; (split; [reflexivity|intro Contra; discriminate]).
+
+  eexists. exact EE.
+Qed.
+
+Ltac concretize_delta HD v :=
+  lazymatch type of HD with has_delta ?vd ?h ?s0 ?s1 ?δ =>
+  lazymatch eval compute in (δ<{vd}>[[v]]) with
+  | Some ?e =>
+      let EE := fresh in
+      mk_eval_exp h s0 e EE; [|
+          let SV := fresh "Hsv" in
+          einstantiate trivial (HD v) as SV; clear EE]
+  | None => fail "Unknown value for " v
+  end
+  end.
+
+Require Import mod_arith.
+
+Theorem getmem_frame_absdist: forall e1 e2 len1 len2 m a1 a2 v,
+  len1 <= absdist a1 a2 -> len2 <= absdist a1 a2 ->
+  getmem e1 len1 (setmem e2 len2 m a2 v) a1 = getmem e1 len1 m a1.
+Proof.
+  unfold absdist. intros. destruct (_ <=? _) eqn: LE.
+  - apply N.leb_le in LE. specialize (conv_le_add_le_sub_r _ _ _ H LE). intro.
+    apply getmem_frame_low. rewrite N.add_comm. assumption.
+  - apply not_true_iff_false in LE. assert (a2 < a1).
+    apply N.lt_nge. revert LE. contrapositive N.leb_le.
+    apply getmem_frame_high. rewrite N.add_comm. apply conv_le_add_le_sub_r.
+    assumption. intros X. rewrite H1 in X. discriminate.
+Qed.
+
+Theorem my_prog_nwc: forall s2 s1, my_prog s1 = my_prog s2.
+Proof. reflexivity. Qed.
+
+Theorem my_prog_hints_correct: forall esp0 mem s0 ts evs
+  (ESP0: s0 R_ESP = Ⓓ esp0) (MEM0: s0 V_MEM32 = Ⓜmem) (ESP_BIG: 8 <= esp0)
+  (RET: my_prog s0 (mem Ⓓ[ esp0 ]) = None) (WM: forall s0, s0 A_WRITE = Ⓜ (fun _ => 1))
+  (RM: forall s0, s0 A_READ = Ⓜ (fun _ => 1))
+  (MDL0: models x86typctx s0) (MPT: my_prog_trace 100 = Some (ts, false, evs)),
+  sat_evidences evs my_prog fh 0 s0.
+Proof.
+  intros. vm_compute in MPT. inversion MPT. subst. clear MPT.
+  repeat constructor. eassert (MDL': models _ s1).
+    eapply preservation_exec_stmt; [| |exact XS0].
+    eapply preservation_exec_prog; [|exact my_prog_welltyped|]; eassumption.
+    eapply typchk_stmt_sound; reflexivity. simpl in MDL'.
+
+  step_stmt XS. destruct XS as [ [? ?] ? ]. inversion H0. subst.
+
+  concretize_delta HD (V_TEMP 6).
+
+  (* Prove memory accesses *)
+  repeat split; try reflexivity; unfold mem_readable, mem_writable; psimpl;
+  eexists; (split; [apply WM + apply RM|intro Contra; discriminate]).
+
+  psimpl in Hsv1. rewrite Hsv1 in Hsv. remember (2 ^ 32). inversion Hsv.
+  subst. repeat unsimpl (getmem LittleE 4 _ _). repeat unsimpl (setmem LittleE 4 _ _).
+  specialize (x86_regsize MDL0 ESP0) as ESP_BND. cbv beta match delta [x86typctx] in ESP_BND.
+
+  assert (4 <= 2 ^ 32 + esp0). apply le_le_add_r. discriminate.
+  assert (EQ_ESP0: 2 ^ 32 + esp0 - 4 ⊕ 4 = esp0).
+  rewrite <- N.add_sub_swap, <- N.add_sub_assoc, N.sub_diag, N.add_0_r,
+    N.add_mod, N.mod_same, N.add_0_l, N.mod_mod, N.mod_small by trivial2.
+  reflexivity. rewrite EQ_ESP0.
+
+  (* Figure the modular arithmetic stuff *)
+  assert (2 ^ 32 - 4 ⊕ esp0 < 2 ^ 32). apply N.mod_lt. discriminate.
+  assert (2 ^ 32 - 4 + esp0 ⊕ 4294967292 < 2 ^ 32). apply N.mod_lt. discriminate.
+  assert (4 <= absdist esp0 (2 ^ 32 + esp0 ⊖ 4)).
+    erewrite N.add_sub_swap, <- modabsdist_eq_absdist, modr_modabsdist by trivial2.
+    einversion trivial (modabsdist_add_l (2 ^ 32)) as [MAD|MAD];
+        rewrite MAD; discriminate.
+  assert (4 <= absdist esp0 (2 ^ 32 + esp0 - 4 ⊕ 4294967292)).
+    erewrite N.add_sub_swap, <- modabsdist_eq_absdist, modr_modabsdist by trivial2.
+    rewrite <- N.add_assoc, (N.add_comm esp0), N.add_assoc.
+    einversion trivial (modabsdist_add_l (2 ^ 32)) as [MAD|MAD];
+        rewrite MAD; discriminate.
+
+  repeat rewrite getmem_frame_absdist; trivial2.
+Qed.
 
 Definition ret_pres (esp0:N) (mem:addr->N) (s:store) :=
   exists mem1, s V_MEM32 = Ⓜ mem1 /\ mem Ⓓ[ esp0 ] = mem1 Ⓓ[ esp0 ].
@@ -1277,14 +1470,6 @@ Definition strchr_trace_hint (p: program) (a: addr) (ts: trace_states):
 Require Extraction.
 Extraction Language OCaml.
 
-Definition domain1 var :=
-  match var with
-  | V_TEMP _ => false
-  | R_AF | R_CF | R_DF | R_OF | R_PF | R_SF | R_ZF => false
-  | R_EAX | R_ECX | R_EDX => false
-  | _ => true
-  end.
-
 Definition strchr_trace reachables := expand_trace_program_n 100 (fun _ => true)
   strchr_trace_hint strchr_i386 reachables (tupdate_n treeN_nil 0 nil).
 
@@ -1309,7 +1494,9 @@ Proof.
   | Some (?v, nil) => clear x; pose (reachables := v)
   end.
   pose (x := strchr_trace2 (list_to_set reachables)).
-  time (vm_compute in x).
+  time (vm_compute in x). unbox_res x.
+
+  pose (y := tget_n x 401); compute in y.
 
   pose (x := match strchr_trace reachables with
              | Some (ts, b) =>
